examples/find/find_spec.v
@@ -27,33 +27,33 @@ Axiom le_f_N : `f <= N`.
 (* Specification part *)
 
 Definition n_invariant :=
-  [n:Z][A:(array (Zs N) Z)]
+  [n:Z][A:(array Z)]
      `f <=n`
   /\ (p,q:Z)(`1<=p` -> `p<=n` -> `n<q` -> `q<=N` -> (Zle #A[p] #A[q])).
 
 Definition m_invariant :=
-  [m:Z][A:(array (Zs N) Z)]
+  [m:Z][A:(array Z)]
      (Zle m f)
   /\ (p,q:Z)(`1<=p` -> `p<m` -> `m<=q` -> `q<=N` -> (Zle #A[p] #A[q])).
 
 Definition i_invariant :=
-  [m,n,i,r:Z][A:(array (Zs N) Z)]
+  [m,n,i,r:Z][A:(array Z)]
      (Zle m i)
   /\ ((p:Z)(`1<=p` -> `p<i` -> (Zle #A[p] r)))
   /\ (`i<=n` -> (EX p:Z | `i<=p` /\ `p<=n` /\ (Zle r #A[p]))).
   
 Definition j_invariant :=
-  [m,n,j,r:Z][A:(array (Zs N) Z)]
+  [m,n,j,r:Z][A:(array Z)]
      (Zle j n)
   /\ ((q:Z)(`j<q` -> `q<=N` -> (Zle r #A[q])))
   /\ (`m<=j` -> (EX q:Z | `m<=q` /\ `q<=j` /\ (Zle #A[q] r))).
 
 Definition termination :=
-  [i,j,i0,j0,r:Z][A:(array (Zs N) Z)]
+  [i,j,i0,j0,r:Z][A:(array Z)]
     (`i>i0` /\ `j<j0`) \/ (`i<=f<=j` /\ #A[f]=r).
 
 Definition found :=
-  [A:(array (Zs N) Z)]
+  [A:(array Z)]
     (p,q:Z)`1<=p` -> `p<=f` -> `f<=q` -> `q<=N` 
       	     -> (Zle #A[p] #A[f]) /\ (Zle #A[f] #A[q]).
 
